theories/lang/cpp/logic/wp.v
@@ -12,7 +12,7 @@ Require Import iris.bi.monpred.
 Require Import bedrock.lang.proofmode.proofmode.
 Require Import iris.proofmode.classes.
 
-Require Import bedrock.lang.cpp.ast.
+Require Import bedrock.lang.cpp.syntax.
 Require Import bedrock.lang.cpp.semantics.
 Require Import bedrock.lang.cpp.logic.pred.
 Require Import bedrock.lang.cpp.logic.heap_pred.
@@ -40,6 +40,7 @@ Module FreeTemps.
   Inductive t : Set :=
   | id (* = fun x => x *)
   | delete (ty : decltype) (p : ptr) (* = delete_val ty p *)
+           (* ^^ this type has qualifiers but is otherwise a runtime type *)
   | delete_va (va : list (type * ptr)) (p : ptr)
   | seq (f g : t) (* = fun x => f $ g x *)
   | par (f g : t) (* = fun x => Exists Qf Qg, f Qf ** g Qg ** (Qf -* Qg -* x) *)
@@ -1253,13 +1254,13 @@ Section with_cpp.
    * note: the [list ptr] will be related to the register set.
    *)
   Parameter wp_fptr
-    : forall (tt : type_table) (fun_type : functype)
+    : forall (tt : type_table) (fun_type : type) (* TODO: function type *)
         (addr : ptr) (ls : list ptr) (Q : ptr -> epred), mpred.
 
   Axiom wp_fptr_complete_type : forall te ft a ls Q,
       wp_fptr te ft a ls Q
       |-- wp_fptr te ft a ls Q **
-          [| exists cc ar tret targs, ft = Tfunction (cc:=cc) (ar:=ar) tret targs |].
+          [| exists cc ar tret targs, ft = Tfunction (@FunctionType _ cc ar tret targs) |].
 
   (* A type is callable against a type table if all of its arguments and return
      type are [complete_type]s.
@@ -1267,11 +1268,11 @@ Section with_cpp.
      This effectively means that there is enough information to determine the
      calling convention.
    *)
-  Definition callable_type (tt : type_table) (t : functype) : Prop :=
+  Definition callable_type (tt : type_table) (t : type) : Prop. (* TODO: function type + complete_type
     match t with
-    | Tfunction ret args => complete_type tt ret /\ List.Forall (complete_type tt) args
+    | Tfunction ft => complete_type tt ft.(ft_return) /\ List.Forall (complete_type tt) ft.(ft_args)
     | _ => False
-    end.
+    end. *) Admitted.
 
   (* this axiom states that the type environment for an [wp_fptr] can be
      narrowed as long as the new type environment [small]/[tt2] is smaller than
@@ -1356,7 +1357,7 @@ Section with_cpp.
            exploit this is to use [reinterpret_cast< >] to cast a function pointer
            to an member pointer or vice versa.
    *)
-  Definition mspec (tt : type_table) (this_type : exprtype) (fun_type : functype)
+  Definition mspec (tt : type_table) (this_type : exprtype) (fun_type : type)
     : ptr -> list ptr -> (ptr -> epred) -> mpred :=
     wp_fptr tt (Tmember_func this_type fun_type).
 
