theories/lang/cpp/parser/decl.v
@@ -4,18 +4,21 @@
  * See the LICENSE-BedRock file in the repository root for details.
  *)
 
-Require Import bedrock.lang.cpp.parser2.prelude.
-Require Import bedrock.lang.cpp.parser2.lang.
-Import LangNotations.
+Require Import bedrock.lang.cpp.parser.prelude.
+Require Import bedrock.lang.cpp.parser.lang.
 
 (** * Derived declaration helpers emitted by cpp2v *)
 
 Module ParserDecl (Import Lang : PARSER_LANG).
-  #[local] Notation obj_name := (obj_name parser_lang).
+  #[local] Notation obj_name := (obj_name' parser_lang).
 
   Definition pure_virt (on : obj_name) : obj_name * option obj_name :=
     (on, None).
   Definition impl_virt (on : obj_name) : obj_name * option obj_name :=
     (on, Some on).
+
+  (* This is used for base classes. *)
+  Definition mkBase (on : classname' parser_lang) (li : LayoutInfo) : classname' parser_lang * LayoutInfo :=
+    (on, li).
 
 End ParserDecl.
