tests/cpp2v/name_test_id.t/run.t
@@ -8,24 +8,23 @@
   
   Definition module_names : list Mname :=
     (
-      (Nscoped
-        (Nglobal (Nid "ns")) (Nid "inhabit")) ::
+      (* CXXRecord ns::inhabit at $TESTCASE_ROOT/test.cpp:10:5 *) (Nscoped (Nglobal (Nid "ns")) (Nid "inhabit")) ::
   
-      (Nglobal (Nid "c")) ::
+      (* CXXRecord c at $TESTCASE_ROOT/test.cpp:12:1 *) (Nglobal (Nid "c")) ::
   
-      (Nglobal (Nid "s")) ::
+      (* CXXRecord s at $TESTCASE_ROOT/test.cpp:13:1 *) (Nglobal (Nid "s")) ::
   
-      (Nglobal (Nid "u")) ::
+      (* CXXRecord u at $TESTCASE_ROOT/test.cpp:14:1 *) (Nglobal (Nid "u")) ::
   
-      (Nglobal (Nid "e1")) ::
+      (* Enum e1 at $TESTCASE_ROOT/test.cpp:15:1 *) (Nglobal (Nid "e1")) ::
   
-      (Nglobal (Nid "e2")) ::
+      (* Enum e2 at $TESTCASE_ROOT/test.cpp:16:1 *) (Nglobal (Nid "e2")) ::
   
-      (Nglobal (Nid "t1")) ::
+      (* Typedef t1 at $TESTCASE_ROOT/test.cpp:17:1 *) (Nglobal (Nid "t1")) ::
   
-      (Nglobal (Nid "t2")) ::
+      (* TypeAlias t2 at $TESTCASE_ROOT/test.cpp:18:1 *) (Nglobal (Nid "t2")) ::
   
-      (Nglobal (Nid "v")) ::
+      (* Var v at $TESTCASE_ROOT/test.cpp:19:1 *) (Nglobal (Nid "v")) ::
       nil).
   
   Definition template_names : list Mname :=
